arm+arm-hyp+aarch64 machine: cacheLineBits from kernel config
Use generated CONFIG_L1_CACHE_LINE_SIZE_BITS as source of truth for
the value of cacheLineBits

The requirements for cacheLineBits are numeric: we need more than 1 and
less than or equal to ptBits, which is only available as a constant
after ExecSpec.

1 is excluded, because we want to be able to fold the value of
cacheLineBits inside C cache operations, and 1 is mentioned as index
increment. No other numerals conflict in these functions.

The only observed values for cacheLineBits are 5 and 6 on Arm, but
there is no need to be more restrictive than cacheLineBits_sanity.

Signed-off-by: Gerwin Klein <gerwin.klein@proofcraft.systems>

spec/machine/ARM_HYP/Platform.thy
@@ -43,7 +43,7 @@ definition pageColourBits :: nat where
   "pageColourBits \<equiv> 2"
 
 definition cacheLineBits :: nat where
-  "cacheLineBits = 6"
+  "cacheLineBits = CONFIG_L1_CACHE_LINE_SIZE_BITS"
 
 definition cacheLine :: nat where
   "cacheLine = 2^cacheLineBits"
